partial commit for victor

src/Network.thy
@@ -14,12 +14,12 @@ locale infinite_event_structure =
   fixes carriers :: "nat \<Rightarrow> 'a event set"
   fixes node_total_order :: "'a event \<Rightarrow> nat \<Rightarrow> 'a event \<Rightarrow> bool" (infix "\<sqsubset>\<^sup>_" 50)
   fixes global_order :: "'a event \<Rightarrow> 'a event \<Rightarrow> bool" (infix "\<sqsubset>\<^sup>G" 50 )
-  assumes global_order_trans: "{e1, e2, e3} \<subseteq> (\<Union>i. carriers i) \<Longrightarrow> e1 \<sqsubset>\<^sup>G e2 \<Longrightarrow> e2 \<sqsubset>\<^sup>G e3 \<Longrightarrow> e1 \<sqsubset>\<^sup>G e3"
+  assumes global_order_trans: "e1 \<sqsubset>\<^sup>G e2 \<Longrightarrow> e2 \<sqsubset>\<^sup>G e3 \<Longrightarrow> e1 \<sqsubset>\<^sup>G e3"
   assumes global_order_irrefl: "e1 \<in> (\<Union>i. carriers i) \<Longrightarrow> \<not> (e1 \<sqsubset>\<^sup>G e1)"
-  assumes node_total_order_trans: "{e1, e2, e3} \<subseteq> carriers i \<Longrightarrow> e1 \<sqsubset>\<^sup>i e2 \<Longrightarrow> e2 \<sqsubset>\<^sup>i e3 \<Longrightarrow> e1 \<sqsubset>\<^sup>i e3"
+  assumes node_total_order_trans: "e1 \<sqsubset>\<^sup>i e2 \<Longrightarrow> e2 \<sqsubset>\<^sup>i e3 \<Longrightarrow> e1 \<sqsubset>\<^sup>i e3"
   assumes node_total_order_total: "{e1, e2} \<subseteq> carriers i \<Longrightarrow> e1 \<noteq> e2 \<Longrightarrow> (e1 \<sqsubset>\<^sup>i e2) \<or> (e2 \<sqsubset>\<^sup>i e1)"
   assumes node_total_order_irrefl: "e1 \<in> carriers i \<Longrightarrow> \<not> (e1 \<sqsubset>\<^sup>i e1)"
-  assumes local_order_to_global: "{e1, e2} \<subseteq> carriers i \<Longrightarrow> e1 \<sqsubset>\<^sup>i e2 \<Longrightarrow> e1 \<sqsubset>\<^sup>G e2"
+  assumes local_order_to_global: "e1 \<sqsubset>\<^sup>i e2 \<Longrightarrow> e1 \<sqsubset>\<^sup>G e2"
   assumes global_order_to_local: "{e1, e2} \<subseteq> carriers i \<Longrightarrow> e1 \<sqsubset>\<^sup>G e2 \<Longrightarrow> e1 \<sqsubset>\<^sup>i e2"
   assumes local_order_carrier_closed: "e1 \<sqsubset>\<^sup>i e2 \<Longrightarrow> {e1,e2} \<subseteq> carriers i"
   assumes global_order_carrier_closed: "e1 \<sqsubset>\<^sup>G e2 \<Longrightarrow> {e1, e2} \<subseteq> (\<Union>i. carriers i)"
@@ -29,9 +29,10 @@ locale infinite_event_structure =
   assumes carriers_message_consistent: "(j, bt, m) \<in> carriers i \<Longrightarrow> i = j"
   assumes broadcast_fifo_order: "{(j, Deliver, m1), (j, Deliver, m2)} \<subseteq> carriers j \<Longrightarrow> (i, Broadcast, m1) \<sqsubset>\<^sup>i (i, Broadcast, m2) \<Longrightarrow> (j, Deliver, m1) \<sqsubset>\<^sup>j (j, Deliver, m2)"
   assumes broadcast_causal: "{(j, Deliver, m1), (j, Deliver, m2)} \<subseteq> carriers j \<Longrightarrow> (i, Deliver, m1) \<sqsubset>\<^sup>i (i, Broadcast, m2) \<Longrightarrow> (j, Deliver, m1) \<sqsubset>\<^sup>j (j, Deliver, m2)"
+  assumes broadcasts_unique: "i \<noteq> j \<Longrightarrow> (i, Broadcast, m) \<in> carriers i \<Longrightarrow> \<not> (j, Broadcast, m) \<in> carriers j"
 
 interpretation trivial_model: infinite_event_structure "\<lambda>m. {}" "\<lambda>e1 m e2. False" "\<lambda>e1 e2. False"
-  by standard simp_all
+  by standard auto
 
 interpretation non_trivial_model: infinite_event_structure
   "\<lambda>m. if m = 0 then {(0, Broadcast, id), (0, Deliver, id)} else {(m, Deliver, id)}"
@@ -42,10 +43,99 @@ interpretation non_trivial_model: infinite_event_structure
 locale finite_event_structure = infinite_event_structure +
   assumes finite_carriers: "finite (carriers i)"
 
+context finite_event_structure begin
+
+definition hb :: "('a \<Rightarrow> 'a) \<Rightarrow> ('a \<Rightarrow> 'a) \<Rightarrow> bool" where
+  "hb m1 m2 \<equiv> (\<exists>i. ((i, Broadcast, m1) \<sqsubset>\<^sup>i (i, Broadcast, m2) \<or>
+                  (i, Deliver, m1) \<sqsubset>\<^sup>i (i, Broadcast, m2)))"
+
+definition weak_hb :: "('a \<Rightarrow> 'a) \<Rightarrow> ('a \<Rightarrow> 'a) \<Rightarrow> bool" where
+  "weak_hb m1 m2 \<equiv> hb m1 m2 \<or> m1 = m2"
+
+sublocale hb: happens_before weak_hb hb
+proof
+  fix x y
+  show "hb x y = (weak_hb x y \<and> \<not> weak_hb y x)"
+  unfolding hb_def weak_hb_def
+    apply standard
+    apply(erule exE)
+    apply(erule disjE)
+    apply(rule conjI)
+    apply(rule disjI1)
+    apply(rule_tac x=i in exI, simp)
+    apply(rule notI)
+    apply(erule disjE)
+    apply(erule exE)
+    apply(erule disjE)
+    apply(case_tac "i=ia")
+    apply clarsimp
+    using node_total_order_irrefl node_total_order_trans
+      local_order_carrier_closed insert_subset apply blast
+    using broadcasts_unique apply(meson insert_subset local_order_carrier_closed)
+    apply(case_tac "i=ia")
+    apply clarsimp
+    using broadcast_before_delivery local_order_carrier_closed node_total_order_trans apply(smt infinite_event_structure.global_order_to_local infinite_event_structure_axioms insert_subset node_total_order_irrefl)
+    apply(drule local_order_carrier_closed)+
+    using broadcasts_unique apply(meson insert_subset)
+    apply(frule local_order_carrier_closed)
+    using node_total_order_irrefl apply simp
+    apply(frule local_order_carrier_closed; clarsimp)
+    apply(frule delivery_has_a_cause)
+    apply(frule broadcast_causal[rotated], clarsimp)
+    apply(rule conjI, assumption)
+    apply(rule no_message_lost, assumption)
+    apply(rule conjI)
+    apply(erule exE)
+    apply force
+    apply(erule exE)
+    apply(rule conjI)
+    apply clarsimp
+    apply(rule conjI)
+    apply(rule notI)
+    apply(frule local_order_carrier_closed)
+    apply(frule local_order_carrier_closed) back
+    apply(drule broadcast_fifo_order[rotated], clarsimp)
+    apply(rule conjI, assumption, assumption)
+    using node_total_order_irrefl apply (meson insert_subset node_total_order_trans)
+    apply(rule notI)
+    using broadcast_before_delivery apply (meson global_order_to_local global_order_trans insert_subset local_order_carrier_closed local_order_to_global node_total_order_irrefl)
+    apply clarsimp
+    using node_total_order_irrefl apply blast
+    apply(erule conjE)
+    apply(erule disjE)
+    apply(erule exE)
+    apply clarsimp
+    apply(erule disjE)
+    apply force
+    apply force
+    apply clarsimp
+  done
+next
+  fix x
+  show "weak_hb x x"
+  unfolding weak_hb_def by force
+next
+  fix x y z
+  assume "weak_hb x y" "weak_hb y z"
+  thus "weak_hb x z"
+  unfolding weak_hb_def hb_def
+    apply -
+    apply safe
+    apply (metis (mono_tags, hide_lams) broadcasts_unique insert_subset local_order_carrier_closed node_total_order_trans)
+    apply (meson broadcast_fifo_order insert_subset local_order_carrier_closed no_message_lost node_total_order_trans)
+    apply (metis (no_types, lifting) broadcasts_unique insert_subset local_order_carrier_closed node_total_order_trans)
+    apply (meson broadcast_causal delivery_has_a_cause insert_subset local_order_carrier_closed no_message_lost node_total_order_trans)
+    apply blast
+    apply blast
+  done
+qed
+
+end
+
 definition (in finite_event_structure) ordered_node_events :: "nat \<Rightarrow> 'a event list" where
   "ordered_node_events i \<equiv>
      let events = carriers i in
-       linorder.sorted_list_of_set (\<lambda>e1 e2. e1 \<sqsubset>\<^sup>i e2)
+       linorder.sorted_list_of_set (\<lambda>e1 e2. e1 \<sqsubset>\<^sup>i e2 \<or> e1 = e2)
          (Set.filter (\<lambda>e.
             case e of (_, Broadcast, _) \<Rightarrow> HOL.False | (_, Deliver, _) \<Rightarrow> HOL.True) events)"
 
